mem/MemOpen.v
@@ -24,17 +24,18 @@ Let _memRA: URA.t := (mblock ==> Z ==> (Excl.t val))%ra.
 
 Section TUNNEL.
   Context `{Σ: GRA.t}.
-  Definition mk_tunneled {X: Type} (PQ: X -> ((Any.t -> ord -> iProp) * (Any.t -> iProp))): fspec :=
+  Definition mk_tunneled {X: Type} (DPQ: X -> ((ord * (Any.t -> iProp)) * (Any.t -> iProp))): fspec :=
     (* mk_fspec (fun _ x y a o => (((fst ∘ PQ) x a o: iProp) ∧ ⌜y = tt↑⌝)%I) *)
     (*          (fun _ x z a => (((snd ∘ PQ) x a: iProp) ∧ ⌜z = tt↑⌝)%I) *)
-    mk_fspec (fun _ x y a o =>
+    mk_fspec (fun x => match x with | Some x => (fst ∘ fst ∘ DPQ) x | _ => ord_top end)
+             (fun _ x y a =>
                 match x with
-                | Some x => (((fst ∘ PQ) x a o: iProp))%I
-                | _ => ⌜y = a ∧ o = ord_top⌝%I: iProp
+                | Some x => (((snd ∘ fst ∘ DPQ) x a: iProp))%I
+                | _ => ⌜y = a⌝%I: iProp
                 end)
              (fun _ x z a =>
                 match x with
-                | Some x => (((snd ∘ PQ) x a: iProp))%I
+                | Some x => (((snd ∘ DPQ) x a: iProp))%I
                 | _ => ⌜z = a⌝%I: iProp
                 end)
   .
@@ -48,40 +49,40 @@ Section PROOF.
 
   Definition alloc_spec: fspec :=
     (mk_tunneled (fun sz => (
-                     (fun varg o => (⌜varg = [Vint (Z.of_nat sz)]↑ /\ (8 * (Z.of_nat sz) < modulus_64)%Z /\ o = ord_pure 0⌝)%I),
-                     (fun vret => (∃ b, ⌜vret = (Vptr b 0)↑⌝ **
-                                        OwnM ((b, 0%Z) |-> (List.repeat Vundef sz)))%I)
+                      (ord_pure 0),
+                      (fun varg => (⌜varg = [Vint (Z.of_nat sz)]↑ /\ (8 * (Z.of_nat sz) < modulus_64)%Z⌝)%I),
+                      (fun vret => (∃ b, ⌜vret = (Vptr b 0)↑⌝ **
+                                                           OwnM ((b, 0%Z) |-> (List.repeat Vundef sz)))%I)
     ))).
 
   Definition free_spec: fspec :=
     (mk_tunneled (fun '(b, ofs) => (
-                     (fun varg o => (∃ v, ⌜varg = ([Vptr b ofs])↑⌝ **
-                                          OwnM ((b, ofs) |-> [v]) **
-                                          ⌜o = ord_pure 0⌝)%I),
-                     (fun vret => ⌜vret = (Vint 0)↑⌝%I)
+                      (ord_pure 0),
+                      (fun varg => (∃ v, ⌜varg = ([Vptr b ofs])↑⌝ ** OwnM ((b, ofs) |-> [v]))%I),
+                      (fun vret => ⌜vret = (Vint 0)↑⌝%I)
     ))).
 
   Definition load_spec: fspec :=
     (mk_tunneled (fun '(b, ofs, v) => (
-                     (fun varg o => ⌜varg = ([Vptr b ofs])↑⌝ **
-                                    OwnM ((b, ofs) |-> [v]) **
-                                    ⌜o = ord_pure 0⌝),
-                     (fun vret => OwnM ((b, ofs) |-> [v]) ** ⌜vret = v↑⌝)
+                      (ord_pure 0),
+                      (fun varg => ⌜varg = ([Vptr b ofs])↑⌝ ** OwnM ((b, ofs) |-> [v])),
+                      (fun vret => OwnM ((b, ofs) |-> [v]) ** ⌜vret = v↑⌝)
     ))).
 
   Definition store_spec: fspec :=
     (mk_tunneled
        (fun '(b, ofs, v_new) => (
-            (fun varg o =>
-               (∃ v_old, ⌜varg = ([Vptr b ofs ; v_new])↑⌝ **
-                          OwnM ((b, ofs) |-> [v_old]) ** ⌜o = ord_pure 0⌝)%I),
+            (ord_pure 0),
+            (fun varg =>
+               (∃ v_old, ⌜varg = ([Vptr b ofs ; v_new])↑⌝ ** OwnM ((b, ofs) |-> [v_old]))%I),
             (fun vret => OwnM ((b, ofs) |-> [v_new]) ** ⌜vret = (Vint 0)↑⌝)
     ))).
 
   Definition cmp_spec: fspec :=
     (mk_tunneled
        (fun '(result, resource) => (
-          (fun varg o =>
+            (ord_pure 0),
+          (fun varg =>
           ((∃ b ofs v, ⌜varg = [Vptr b ofs; Vnullptr]↑⌝ ** ⌜resource = ((b, ofs) |-> [v])⌝ ** ⌜result = false⌝) ∨
            (∃ b ofs v, ⌜varg = [Vnullptr; Vptr b ofs]↑⌝ ** ⌜resource = ((b, ofs) |-> [v])⌝ ** ⌜result = false⌝) ∨
            (∃ b0 ofs0 v0 b1 ofs1 v1, ⌜varg = [Vptr b0 ofs0; Vptr b1 ofs1]↑⌝ **
@@ -89,7 +90,6 @@ Section PROOF.
            (∃ b ofs v, ⌜varg = [Vptr b ofs; Vptr b  ofs]↑⌝ ** ⌜resource = ((b, ofs) |-> [v])⌝ ** ⌜result = true⌝) ∨
            (⌜varg = [Vnullptr; Vnullptr]↑ /\ result = true⌝))
             ** OwnM(resource)
-            ** ⌜o = ord_pure 0⌝
           ),
           (fun vret => OwnM(resource) ** ⌜vret = (if result then Vint 1 else Vint 0)↑⌝)
     ))).
